Isabelle/SafetyOracle.thy
@@ -1,93 +1,81 @@
 theory SafetyOracle
 
-imports Main CBCCasper ConsensusSafety
+imports Main CBCCasper ConsensusSafety LatestMessage
 
 begin
 
 (* Section 7: Safety Oracles *)
 (* Section 7.1 Preliminary Definitions *)
 
-(* Definition 7.1 *)
-fun later :: "(message * message) \<Rightarrow> bool"
-  where
-    "later (m1, m2) = (m2 \<in> justification m1)"
-
-(* Definition 7.2 *)
-fun (in Protocol) from_sender :: "(validator * state) \<Rightarrow> message set"
-  where
-    "from_sender (v, \<sigma>) = {m \<in> M. m \<in> \<sigma> \<and> sender m = v}"
-     
-(* Definition 7.3 *)
-fun (in Protocol) later_from :: "(message * validator * state) \<Rightarrow> message set"
-  where
-    "later_from (m, v, \<sigma>) = {m' \<in> M. m \<in> \<sigma> \<and> sender m' = v \<and> later (m', m)}"
- 
-(* Definition 7.4 *)
-fun (in Protocol) latest_messages :: "(state * validator) \<Rightarrow> message set"
-  where
-    "latest_messages (\<sigma>, v) = {m \<in> M. m \<in> \<sigma> \<and> sender m = v \<and> later_from (m, v, \<sigma>) = \<emptyset>}"
-
-(* Definition 7.5 *)
-fun (in Protocol) latest_messages_from_honest_validators :: "(state * validator) \<Rightarrow> message set"
-  where
-    "latest_messages_from_honest_validators (\<sigma>, v) = 
-      (if v \<in> equivocating_validators \<sigma> then \<emptyset> else latest_messages (\<sigma>, v))"
-
-(* Definition 7.6 *)
-fun (in Protocol) latest_estimates_from_honest_validators:: "(state * validator) \<Rightarrow> consensus_value set"
-  where
-    "latest_estimates_from_honest_validators (\<sigma>, v) = 
-      {est m | m. m \<in> latest_messages_from_honest_validators (\<sigma>, v)}"
-
-lemma (in Protocol) latest_estimates_from_honest_validators_type :
-  "\<forall> \<sigma> v. \<sigma> \<in> \<Sigma> \<and> v \<in> V \<longrightarrow> latest_estimates_from_honest_validators (\<sigma>, v) \<subseteq> C"
-  using M_type by auto
+(* NOTE: Definition 7.1 is replaced by definition 4.2*)
+(* NOTE: Definition 7.2 is duplicate of definition 4.3 *)
+(* NOTE: Definition 7.3 is duplicate of definition 4.5 *)
+(* NOTE: Definition 7.4 is duplicate of definition 4.6 *)
+(* NOTE: Definition 7.5 is duplicate of definition 4.11 *)
+(* NOTE: Definition 7.6 is duplicate of definition 4.13 *)
 
 (* Definition 7.7 *)
-fun (in Protocol) latest_justifications_from_honest_validators :: "(state * validator) \<Rightarrow> state set"
+fun latest_justifications_from_non_equivocating_validators :: "state \<Rightarrow> validator \<Rightarrow> state set"
   where
-    "latest_justifications_from_honest_validators (\<sigma>, v) = 
-      {justification m | m. m \<in> latest_messages_from_honest_validators (\<sigma>, v)}"
+    "latest_justifications_from_non_equivocating_validators \<sigma> v = 
+      {justification m | m. m \<in> latest_messages_from_non_equivocating_validators \<sigma> v}"
 
-lemma (in Protocol) latest_justifications_from_honest_validators_type :
-  "\<forall> \<sigma> v. \<sigma> \<in> \<Sigma> \<and> v \<in> V \<longrightarrow> latest_justifications_from_honest_validators (\<sigma>, v) \<subseteq> \<Sigma>"
-  using M_type by auto
+lemma (in Protocol) latest_justifications_from_non_equivocating_validators_type :
+  "\<forall> \<sigma> v. \<sigma> \<in> \<Sigma> \<and> v \<in> V \<longrightarrow> latest_justifications_from_non_equivocating_validators \<sigma> v \<subseteq> \<Sigma>"
+  using M_type latest_messages_from_non_equivocating_validators_type by auto
 
 (* Definition 7.8 *)
-fun (in Protocol) agreeing_validators :: "(consensus_value_property * state) \<Rightarrow> validator set"
+(* NOTE: Modified from the original draft. *)
+fun observed_non_equivocating_validators :: "state \<Rightarrow> validator set"
   where
-    "agreeing_validators (p, \<sigma>) = {v \<in> V. \<forall> c \<in> C. c \<in> latest_estimates_from_honest_validators (\<sigma>, v) \<and> p c}"
+    "observed_non_equivocating_validators \<sigma> = observed \<sigma> - equivocating_validators \<sigma>"
+
+fun  agreeing_validators :: "(consensus_value_property * state) \<Rightarrow> validator set"
+  where
+    "agreeing_validators (p, \<sigma>) = {v \<in> observed_non_equivocating_validators \<sigma>. \<forall> c \<in> latest_estimates_from_non_equivocating_validators \<sigma> v. p c}"
+
+lemma (in Protocol) agreeing_validators_type :
+  "\<forall> \<sigma> \<in> \<Sigma>. agreeing_validators (p, \<sigma>) \<subseteq> V"
+  using oberved_type by auto
 
 (* Definition 7.9 *)
-fun (in Protocol) disagreeing_validators :: "(consensus_value_property * state) \<Rightarrow> validator set"
+fun disagreeing_validators :: "(consensus_value_property * state) \<Rightarrow> validator set"
   where
-    "disagreeing_validators (p, \<sigma>) = {v \<in> V. \<exists> c \<in> C. c \<in> latest_estimates_from_honest_validators (\<sigma>, v) \<and> \<not> p c}"
+    "disagreeing_validators (p, \<sigma>) = {v \<in> observed_non_equivocating_validators \<sigma>. \<exists> c \<in> latest_estimates_from_non_equivocating_validators \<sigma> v. \<not> p c}"
+
+lemma (in Protocol) disagreeing_validators_type :
+  "\<forall> \<sigma> \<in> \<Sigma>. disagreeing_validators (p, \<sigma>) \<subseteq> V"
+  using oberved_type by auto
 
 (* Definition 7.10 *)
-definition (in Protocol) weight_measure :: "validator set \<Rightarrow> real"
+definition (in Params) weight_measure :: "validator set \<Rightarrow> real"
   where
     "weight_measure v_set = sum W v_set"
 
 (* Definition 7.11 *)
-fun (in Protocol) is_majority :: "(validator set * state) \<Rightarrow> bool"
+fun (in Params) is_majority :: "(validator set * state) \<Rightarrow> bool"
   where
     "is_majority (v_set, \<sigma>) = (weight_measure v_set > (weight_measure V - weight_measure (equivocating_validators \<sigma>)) div 2)"
    
 (* Definition 7.12 *)
-definition (in Protocol) is_majority_driven :: "consensus_value_property \<Rightarrow> bool"
+definition (in AbstractProtocol) is_majority_driven :: "consensus_value_property \<Rightarrow> bool"
   where
-    "is_majority_driven p = (\<forall> \<sigma> c. \<sigma> \<in> \<Sigma> \<and> c \<in> C \<and> is_majority (agreeing_validators (p, \<sigma>), \<sigma>) \<longrightarrow> c \<in> \<epsilon> \<sigma> \<and> p c)"
+    "is_majority_driven p = (\<forall> \<sigma> c. \<sigma> \<in> \<Sigma> \<and> c \<in> C \<and> is_majority (agreeing_validators (p, \<sigma>), \<sigma>) \<longrightarrow> (\<forall> c \<in> \<epsilon> \<sigma>. p c))"
 
 (* Definition 7.13 *)
-definition (in Protocol) is_max_driven :: "consensus_value_property \<Rightarrow> bool"
+definition (in AbstractProtocol) is_max_driven :: "consensus_value_property \<Rightarrow> bool"
   where
     "is_max_driven p =
       (\<forall> \<sigma> c. \<sigma> \<in> \<Sigma> \<and> c \<in> C \<and> weight_measure (agreeing_validators (p, \<sigma>)) > weight_measure (disagreeing_validators (p, \<sigma>)) \<longrightarrow> c \<in> \<epsilon> \<sigma> \<and> p c)"
 
 (* Definition 7.14 *)
-fun (in Protocol) later_disagreeing_messages :: "(consensus_value_property * message * validator * state) \<Rightarrow> message set"
+fun later_disagreeing_messages :: "(consensus_value_property * message * validator * state) \<Rightarrow> message set"
   where 
-    "later_disagreeing_messages (p, m, v, \<sigma>) = {m' \<in> M. m' \<in> later_from (m, v, \<sigma>) \<and> \<not> p (est m')}"
+    "later_disagreeing_messages (p, m, v, \<sigma>) = {m' \<in> later_from (m, v, \<sigma>). \<not> p (est m')}"
+
+lemma (in Protocol) later_disagreeing_messages_type :
+  "\<forall> p \<sigma> v m. \<sigma> \<in> \<Sigma> \<and> v \<in> V \<and> m \<in> M \<longrightarrow> later_disagreeing_messages (p, m, v, \<sigma>) \<subseteq> M"
+  using later_from_type by auto
 
 (* Definition 7.15 *)
 (* `the_elem` is built-in  *)
@@ -95,17 +83,17 @@ fun (in Protocol) later_disagreeing_messages :: "(consensus_value_property * mes
 (* Section 7.2: Validator Cliques *)
 
 (* Definition 7.16: Clique with 1 layers *)
-fun (in Protocol) is_clique :: "(validator set * consensus_value_property * state) \<Rightarrow> bool"
+fun is_clique :: "(validator set * consensus_value_property * state) \<Rightarrow> bool"
  where
    "is_clique (v_set, p, \<sigma>) = 
-     (\<forall> v \<in> v_set. v_set \<subseteq> agreeing_validators (p, the_elem (latest_justifications_from_honest_validators (\<sigma>, v)))
-     \<and>  (\<forall>  v' \<in> v_set. later_disagreeing_messages (p, the_elem (latest_messages_from_honest_validators (the_elem (latest_justifications_from_honest_validators (\<sigma>, v)), v')), v', \<sigma>) = \<emptyset>))"
+     (\<forall> v \<in> v_set. v_set \<subseteq> agreeing_validators (p, the_elem (latest_justifications_from_non_equivocating_validators \<sigma> v))
+     \<and>  (\<forall>  v' \<in> v_set. later_disagreeing_messages (p, the_elem (latest_messages_from_non_equivocating_validators (the_elem (latest_justifications_from_non_equivocating_validators \<sigma> v)) v'), v', \<sigma>) = \<emptyset>))"
 
 
 (* Section 7.3: Cliques Survive Messages from Validators Outside Clique *)
 
 (* Definition 7.17 *)
-abbreviation (in Protocol) minimal_transitions :: "(state * state) set"
+abbreviation (in Params) minimal_transitions :: "(state * state) set"
   where
     "minimal_transitions \<equiv> {(\<sigma>, \<sigma>') | \<sigma> \<sigma>'. \<sigma> \<in> \<Sigma>t \<and> \<sigma>' \<in> \<Sigma>t \<and> is_future_state (\<sigma>', \<sigma>) \<and> \<sigma> \<noteq> \<sigma>'
       \<and> (\<nexists> \<sigma>''. \<sigma>'' \<in> \<Sigma> \<and> is_future_state (\<sigma>'', \<sigma>) \<and> is_future_state (\<sigma>', \<sigma>'') \<and> \<sigma> \<noteq> \<sigma>'' \<and> \<sigma>'' \<noteq> \<sigma>')}"
@@ -124,13 +112,13 @@ lemma (in Protocol) later_from_not_affected_by_minimal_transitions :
   oops
 
 (* Definition 7.18: One layer clique oracle threshold size *) 
-fun (in Protocol) gt_threshold :: "(validator set * state) \<Rightarrow> bool"
+fun (in Params) gt_threshold :: "(validator set * state) \<Rightarrow> bool"
   where
     "gt_threshold (v_set, \<sigma>)
        = (weight_measure v_set > (weight_measure v_set) div 2 + t  - weight_measure (equivocating_validators \<sigma>))"
 
 (* Definition 7.19: Clique oracle with 1 layers *)
-fun (in Protocol) is_clique_oracle :: "(validator set * state * consensus_value_property) \<Rightarrow> bool"
+fun (in Params) is_clique_oracle :: "(validator set * state * consensus_value_property) \<Rightarrow> bool"
   where
     "is_clique_oracle (v_set, \<sigma>, p)
        = (is_clique (v_set - (equivocating_validators \<sigma>), p, \<sigma>) \<and> gt_threshold (v_set - (equivocating_validators \<sigma>), \<sigma>))"
