Isabelle/CodeGeneration.thy
@@ -1,0 +1,68 @@
+theory CodeGeneration
+
+imports Main CBCCasper SafetyOracle TFGCasper
+
+begin
+
+code_printing
+  type_constructor bool => (Haskell) "bool"
+  | constant True => (Haskell) "true"
+  | constant False => (Haskell) "false"
+
+(* FIXME: How can we remove member func? *)
+definition member :: "'a list \<Rightarrow> 'a \<Rightarrow> bool"
+  where
+    [code_abbrev]: "member xs x \<longleftrightarrow> x \<in> set xs"
+
+instantiation consensus_value :: equal
+begin 
+
+definition "HOL.equal (x ::consensus_value) y \<longleftrightarrow> x = y"
+instance  by standard (simp add: equal_consensus_value_def)
+
+end
+
+code_printing
+  class_instance consensus_value :: "HOL.equal" => (Haskell) -
+  (* |type_constructor consensus_value => (Haskell) "Map String String" *)
+
+
+instantiation validator :: equal
+begin 
+
+definition "HOL.equal (x ::validator) y \<longleftrightarrow> x = y"
+instance  by standard (simp add: equal_validator_def)
+
+end
+
+code_printing
+  class_instance validator :: "HOL.equal" => (Haskell) -
+  (* | type_constructor validator => (Haskell) "Map String String" *)
+
+interpretation p: Params V W t \<Sigma> M for V W t \<Sigma> M
+  done
+
+definition "is_clique_oracle = p.is_clique_oracle"
+
+export_code is_clique is_clique_oracle in Haskell
+  module_name SafetyOracle file GeneratedCode
+
+(* 
+FIXME: TFG is just a interpretation of Params
+definition "bc = GhostParams.best_children"
+
+interpretation gp: GhostParams V W t \<Sigma> M genesis "\<Union> (B_i (genesis, block_generator) `\<nat>)" block_generator for V W t \<Sigma> M genesis B block_generator 
+  using GhostParams_def by blast
+
+term gp.best_children
+
+lemma [code]: "bc = gp.best_children"
+
+definition "best_children = gp.best_children"
+
+(* Question2: No code equations for GhostParams.best_children *)
+export_code best_children in Haskell
+  module_name TFGCasper file GeneratedCode
+ *)
+
+end
